\documentclass[a4paper]{jarticle} 
\usepackage[dvips,usenames]{color} 
\usepackage{graphicx}
\usepackage{fancyhdr}
\usepackage{listings}
\usepackage{bm}  % for bmdefine
% \pagestyle{empty}
\topmargin = 0mm
\oddsidemargin = 5mm
\textwidth = 152mm
\textheight = 240mm
\pagestyle{fancyplain}
\renewcommand{\footrulewidth}{0pt}
\renewcommand{\headrulewidth}{0pt}
\bmdefine{\bx}{x}
\bmdefine{\bv}{v}
\bmdefine{\bh}{h}
\makeatletter
\newcommand{\figcaption}[1]{\def\@captype{figure}\caption{#1}}
\newcommand{\tblcaption}[1]{\def\@captype{table}\caption{#1}}
\makeatother

\begin{document}
\lhead{\small 情報システム工学科}
\rhead{\small 2009年4月12日\\塩貝亮宇}
% \cfoot{}
%
%\begin{flushright}%
%2006年 9月 28日
%\end{flushright}
%

\centerline{\Large\gt GBM}

\vskip 5mm
\centerline{\Large\gt T1076006 塩貝亮宇}

\section{GBM}
\begin{eqnarray}
 \sigma(x) &=& \frac{1}{1 + \exp(-x)}\\
\end{eqnarray}
\subsection{GBMBiasIterate}
\begin{eqnarray}
 E(\bv,\bh) &=&
  -\sum_{i=1}^{D} a_i v_i -\sum_{j=1}^{P} b_j h_j\\
 &+&\sum_{i=1}^{D} \sum_{k=i+1}^{D} v_i L_{ik} v_k
  +\sum_{j=1}^{P} \sum_{j=i+1}^{P} h_j J_{jm} h_m
  +\sum_{i=1}^{D} \sum_{j=1}^{P}   v_i W_{ij} h_j\\
 \mu_j &\leftarrow&
  \sigma(
  -  b_j
  + \sum_{i=1}^{D} v_i W_{ij}
  + \sum_{m=1\backslash j}^{P} \mu_m J_{mj}
  )\\
 p(h_j=1 | \bv, \bh_{-j}) &=&
  \sigma(
  - b_j + \sum_{m=1\backslash j}^{P} J_{jm} h_m
  )\\
 p(v_i=1 | \bh, \bv_{-i}) &=&
  \sigma(
  - a_i
  + \sum_{j=1}^{P} W_{ij} h_j 
  + \sum_{k=1}^{D} L_{ik} v_k
  )\\
\end{eqnarray}

\subsection{GBMNoBiasIterate}
\begin{eqnarray}
 E(\bv, \bh) &=&
   \sum_{i=1}^{D} \sum_{k=i+1}^{D} v_i L_{ik} v_k
  +\sum_{j=1}^{P} \sum_{j=i+1}^{P} h_j J_{jm} h_m
  +\sum_{i=1}^{D} \sum_{j=1}^{P}   v_i W_{ij} h_j\\
 \mu_j &\leftarrow&
  \sigma \left(
	   \sum_{i=1}^{D}               v_i W_{ij}
	  +\sum_{m=1\backslash j}^{P} \mu_m J_{mj}
	 \right)\\
 p(h_j=1| \bv, \bh_{-j}) &=&
  \sigma \left(
  \sum_{i=1}^{D} v_i W_{ij}
  + \sum_{m=1\backslash j}^{P} J_{jm} h_m
  \right)\\
 p(v_i=1| \bh, \bv_{-i}) &=&
  \sigma \left(
    \sum_{j=1}^{P} W_{ij} h_j
  + \sum_{k=1\backslash i}^{D} L_{ik} v_k
  \right)\\
\end{eqnarray}

\subsection{GBMNoBiasNoIterate}
\begin{eqnarray}
 E(\bv,\bh) &=&
  -\sum_{i=1}^{D} \sum_{k=i+1}^{D} v_i L_{ik} v_k
  -\sum_{j=1}^{P} \sum_{m=j+1}^{P} h_j J_{jm} h_m
  -\sum_{i=1}^{D} \sum_{j=1  }^{P} v_i W_{ij} h_j\\
 \mu_j &\leftarrow&
  \sigma(
   \sum_{i=1            }^{D} v_i    W_{ij}
  +\sum_{m=1\backslash j}^{P} J_{mj} \mu_j
  )\\
 p(h_j=1 | \bv, \bh_{-j})  &=&
    \sum_{i=1            }^{D} v_i W_{ij}
  + \sum_{m=1\backslash j}^{P} h_j J_{jm}\\
 p(v_i=1 | \bh, \bv_{-i}) &=&
   \sum_{j=1}^{P} W_{ij} h_j
  +\sum_{k=1\backslash i}^{D} v_i L_{ik} 
\end{eqnarray}

\subsection{GBMBiasIterate}
\begin{eqnarray}
 E(\bv,\bh)
 &=& \sum_{i}^{D} a_i v_i +\sum_{j}^{P} b_j h_j\\
 &-& \sum_{i=1}^{D}\sum_{k=i+1}^{D} v_i L_{ik} v_k
  -  \sum_{j=1}^{P}\sum_{m=j+1}^{P} h_j J_{jm} h_m
  -  \sum_{i=1}^{D}\sum_{j=1}^{P} v_i W_{ij} h_j\\
 \mu_j &\leftarrow&
  \sigma(
  b_j 
  + \sum_{i=1            }^{D} v_i W_{ij}
  + \sum_{m=1\backslash j}^{P} \mu_m J_{mj}
  )\\
 p(h_j=1 | \bv, \bh_{-j}) &=&
  \sigma(
  b_j
  +\sum_{i=1            }^{D} v_i W_{ij}
  +\sum_{m=1\backslash j}^{P} J_{jm} h_m
  )\\
 p(v_i=1 |\bh, \bv_{-i}) &=&
  \sigma(
  a_i
  +\sum_{j=1            }^{P} W_{ij} h_j
  +\sum_{k=1\backslash i}^{D} L_{ik} v_k
  )\\
\end{eqnarray}

\subsection{GBMBiasIterate2}
\begin{eqnarray}
 E(\bv,\bh)
  &=& \sum_{i=1}^{D} a_i v_i +\sum_{j=1}^{P} b_j h_j\\
  &-&\sum_{i=1}^{D}\sum_{k=i+1}^{D} v_i L_{ik} v_k
   - \sum_{j=1}^{P}\sum_{m=j+1}^{P} h_j J_{jm} h_m
   - \sum_{i=1}^{D}\sum_{j=1  }^{P} v_i W_{ij} h_j\\
 \mu_j &\leftarrow& 
  \sigma \left(
	  b_j 
 + \sum_{i=1}^{D} a_i v_i
 + \sum_{i=1            }^{D} v_i W_{ij}
 + \sum_{m=1\backslash j}^{P} \mu_m J_{mj}
 \right)\\
 p(h_j=1 | \bv, \bh_{-j}) &=&
  \sigma \left(
    b_j
  +\sum_{i=1}^{D} a_i v_i
  +\sum_{i=1            }^{D} v_i W_{ij}
  +\sum_{m=1\backslash j}^{P} J_{jm} h_m
  \right)\\
 p(v_i=1 |\bh, \bv_{-i}) &=&
  \sigma \left(
  a_i
  +\sum_{j=1}^{P} b_j h_j
  +\sum_{j=1            }^{P} W_{ij} h_j
  +\sum_{k=1\backslash i}^{D} L_{ik} v_k
  \right)\\
\end{eqnarray}

\subsection{GBMBiasIterate3}
\begin{eqnarray}
 E(\bv,\bh)
  &=& \sum_{i}^{D} a_i v_i +\sum_{j}^{P} b_j h_j\\
  &-& \sum_{i=1}^{D}\sum_{k=i+1}^{D} v_i L_{ik} v_k
   -  \sum_{j=1}^{P}\sum_{m=j+1}^{P} h_j J_{jm} h_m
   -  \sum_{i=1}^{D}\sum_{j=1}^{P} v_i W_{ij} h_j\\
 \mu_j &\leftarrow&
 \sigma \left(
   \sum_{i=1}^{D} a_i v_i
 + \sum_{m=1}^{P} b_m h_m
 + \sum_{i=1            }^{D}  v_i W_{ij}
 + \sum_{m=1\backslash j}^{P}\mu_m J_{mj}
 \right)\\
 p(h_j=1 | \bv, \bh_{-j}) &=&
  \sigma \left(
   \sum_{i=1}^{D} a_i v_i
  +\sum_{m=1}^{P} b_m h_m
  +\sum_{i=1            }^{D} v_i W_{ij}
  +\sum_{m=1\backslash j}^{P} J_{jm} h_m
  \right)\\
 p(v_i=1 |\bh, \bv_{-i}) &=&
  \sigma \left(
   \sum_{k=1}^{D} a_k v_k
  +\sum_{j=1}^{P} b_j h_j
  +\sum_{j=1            }^{P} W_{ij} h_j
  +\sum_{k=1\backslash i}^{D} L_{ik} v_k
  \right)\\
\end{eqnarray}


\end{document}


